{
 "cells": [
  {
   "cell_type": "markdown",
   "metadata": {},
   "source": [
    "# Non Independent Variables\n",
    "\n",
    "This lecture is about relations between variables, and how to handle functions that depend on several variables when they are related\n",
    "\n",
    "Example: $f(P, V, T)$ where $PV = nRT$. What is the rate of change f, p and v wrt t or wrt to each others\n",
    "\n",
    "Function of x, y, z, $f(x, y ,z)$ where the variables are related to each other by some equation $g(x, y, z) = c$. Same setup as last lecture, except we don't just concern on maxima and minima but to understand partial derivatives\n",
    "\n",
    "If $g(x, y, z) = c$, then $z = z(x, y)$, what are $\\frac{\\partial z}{\\partial x}, \\frac{\\partial z}{\\partial y}$?\n",
    "\n",
    "\n",
    "Example: $$x^2 + yz + z^3 = 8$$ at (2, 3, 1)\n",
    "\n",
    "Take differential wrt x, y, z\n",
    "\n",
    "$$2x \\ dx + z \\ dy + (y + 3z^2)\\ dz = 0$$\n",
    "\n",
    "Because g = 8, dg = 0. At (2, 3, 1)\n",
    "\n",
    "$$4\\ dx + dy + 6\\ dz = 0$$\n",
    "\n",
    "If we view $z = z(x, y)$\n",
    "\n",
    "$$dz = -\\frac{1}{6} (4\\ dx + dy)$$\n",
    "\n",
    "$$\\frac{\\partial z}{\\partial x} = -\\frac{2}{3}, \\quad \\frac{\\partial z}{\\partial y} = -\\frac{1}{6}$$\n",
    "\n",
    "To get the first expression, we set y constant, dy = 0. Second expression, x is constant, dx is zero\n",
    "\n",
    "In general, $g(x, y, z) = c$, then \n",
    "\n",
    "$$dg = g_x \\ dx + g_y \\ dy + g_z \\ dz = 0$$\n",
    "\n",
    "Solve for dz:\n",
    "\n",
    "$$dz = -\\frac{g_x}{g_z} \\ dx - \\frac{g_y}{g_z} \\ dy$$\n",
    "\n",
    "So, for $\\frac{\\partial z}{\\partial x}$, set y is constant, dy = 0\n",
    "\n",
    "$$dz = -\\frac{g_x}{g_z}\\ dx \\implies \\frac{\\partial z}{\\partial x} = -\\frac{g_x}{g_z}$$\n",
    "\n",
    "Say $f(x, y) = x + y, \\frac{\\partial f}{\\partial x} = 1$\n",
    "\n",
    "Let change variables, $x = u, y = u + v$, then\n",
    "\n",
    "$$f = 2u + v, \\quad \\frac{\\partial f}{\\partial u} = 2$$\n",
    "\n",
    "So $x = u$ but $\\frac{\\partial f}{\\partial x} \\neq \\frac{\\partial f}{\\partial u}$. How to resolve this contradiction?\n",
    "\n",
    "It is because one is keeping y constant and vary x, another is keeping v constant and vary u\n",
    "\n",
    "Need clearer notation:\n",
    "\n",
    "$$\\left(\\frac{\\partial f}{\\partial x}\\right)_y$$\n",
    "\n",
    "means keep y constant\n",
    "\n",
    "$$\\left(\\frac{\\partial f}{\\partial u}\\right)_v$$\n",
    "\n",
    "means keep v constant\n",
    "\n",
    "$$\\left(\\frac{\\partial f}{\\partial x}\\right)_y \\neq \\left(\\frac{\\partial f}{\\partial x}\\right)_v = \\left(\\frac{\\partial f}{\\partial u}\\right)_v$$"
   ]
  },
  {
   "cell_type": "markdown",
   "metadata": {},
   "source": [
    "### Example: Area of Triangle\n",
    "\n",
    "A triangle with area\n",
    "\n",
    "$$A(a, b, \\theta) = \\frac12 ab \\sin \\theta$$\n",
    "\n",
    "Assume it's a right triangle with $a = b\\cos \\theta$ which is the constraint (relation between a, b, theta)\n",
    "\n",
    "Rate of change of $A$ wrt $\\theta$\n",
    "\n",
    "1. Treat $a, b, \\theta$ as independent, \n",
    "\n",
    "$$\\frac{\\partial A}{\\partial \\theta} = \\left(\\frac{\\partial A}{\\partial \\theta}\\right)_{a,b}$$\n",
    "\n",
    "keep a, b fixed\n",
    "\n",
    "$$\\frac{\\partial A}{\\partial \\theta} = \\frac12 a b \\cos \\theta$$\n",
    "\n",
    "2. Keep $a$ constant, $b$ will change $b = b(a, \\theta) = \\frac{a}{\\cos \\theta}$. So that we keep a right angle\n",
    "\n",
    "$$\\left(\\frac{\\partial A}{\\partial \\theta}\\right)_{a}$$\n",
    "\n",
    "3. Keep $b$ constant, $a = a(b, \\theta)$ changes\n",
    "\n",
    "$$\\left(\\frac{\\partial A}{\\partial \\theta}\\right)_{b}$$\n",
    "\n",
    "\n",
    "### Compute $\\left(\\frac{\\partial A}{\\partial \\theta}\\right)_{a}$\n",
    "\n",
    "Method 0: Solve for b, and substitute\n",
    "\n",
    "$a = b\\cos \\theta \\implies b = \\frac{a}{\\cos \\theta} = a \\sec \\theta$\n",
    "\n",
    "$$A = \\frac12 ab\\sin\\theta = \\frac12 \\frac{a^2 \\sin\\theta}{\\cos\\theta} = \\frac12 a^2 \\tan\\theta$$\n",
    "\n",
    "$$\\left(\\frac{\\partial A}{\\partial \\theta}\\right)_{a} = \\frac12 a^2 \\sec^2\\theta$$\n",
    "\n",
    "Two systematic methods:\n",
    "\n",
    "1. Differentials\n",
    "    - Keep a fixed, da = 0\n",
    "    - constraint $a = b\\cos\\theta$\n",
    "    - $da = \\cos\\theta \\ db - b\\sin\\theta \\ d\\theta \\implies \\cos\\theta \\ db = b\\sin\\theta \\ d\\theta \\implies db = b\\tan\\theta \\ d\\theta$\n",
    "    \n",
    "Function, $A = \\frac12 ab\\sin\\theta$, \n",
    "\n",
    "$$dA = \\frac12 b\\sin\\theta \\ da + \\frac12 a \\sin\\theta \\ db + \\frac12 ab \\cos\\theta \\ d\\theta$$\n",
    "\n",
    "This function tells us how dA varies with da, db, $d\\theta$\n",
    "\n",
    "We have the result of da and db, substitute in\n",
    "\n",
    "$$dA = \\frac12 a\\sin\\theta (b \\tan\\theta \\ d\\theta) + \\frac12 ab \\cos\\theta \\ d\\theta = \\frac12 ab (\\sin\\theta \\tan\\theta + \\cos\\theta) \\ d\\theta$$\n",
    "\n",
    "Because $\\sin\\theta \\tan\\theta + \\cos\\theta = \\sec\\theta$\n",
    "\n",
    "$$dA = \\frac12 ab \\sec\\theta \\ d\\theta$$\n",
    "\n",
    "$$\\left(\\frac{\\partial A}{\\partial \\theta}\\right)_{a} = \\frac12 ab \\sec\\theta$$\n",
    "\n",
    "\n",
    "Summary of method 1\n",
    "\n",
    "- Write dA in terms of da, db, $d\\theta$\n",
    "- a is constant, then da = 0\n",
    "- differentiate constraint, solve for db in terms of $d\\theta$\n",
    "- Plug into dA, get answer\n",
    "\n"
   ]
  },
  {
   "cell_type": "markdown",
   "metadata": {},
   "source": [
    "2. Chain Rule\n",
    "\n",
    "$\\left(\\frac{\\partial }{\\partial \\theta}\\right)_{a}$ in formula for $A$\n",
    "\n",
    "$$\\left(\\frac{\\partial A}{\\partial \\theta}\\right)_{a} = A_{\\theta} \\left(\\frac{\\partial \\theta}{\\partial \\theta}\\right)_{a} + A_a \\left(\\frac{\\partial a}{\\partial \\theta}\\right)_{a} + A_b \\left(\\frac{\\partial b}{\\partial \\theta}\\right)_{a}$$\n",
    "\n",
    "$\\left(\\frac{\\partial \\theta}{\\partial \\theta}\\right)_{a} = 1, \\quad \\left(\\frac{\\partial a}{\\partial \\theta}\\right)_{a} = 0, \\quad \\left(\\frac{\\partial b}{\\partial \\theta}\\right)_{a}$ can be found by constraint"
   ]
  },
  {
   "cell_type": "code",
   "execution_count": null,
   "metadata": {},
   "outputs": [],
   "source": []
  }
 ],
 "metadata": {
  "kernelspec": {
   "display_name": "Julia 1.5.0",
   "language": "julia",
   "name": "julia-1.5"
  },
  "language_info": {
   "file_extension": ".jl",
   "mimetype": "application/julia",
   "name": "julia",
   "version": "1.5.0"
  }
 },
 "nbformat": 4,
 "nbformat_minor": 4
}
